KAM

krivineAM.v
@@ -5,7 +5,6 @@ Require Import List.
 Require Import Omega.
 Require Import untypedLambda.
 
-
 (*Krivine Abstract Machine*)
 
 (*Syntax*)
@@ -26,15 +25,17 @@ Definition state := prod (prod code environment) environment.
 
 Check environment_ind.
 
+Check cons (cnil,nul) nul.
+
 (*Semantics*)
 
-Fixpoint exec_inst (s: state): option state:=
+Fixpoint exec_inst (s: state): state:=
   match s with
-    | (cCons (Access 0) c, cons (c0,e0) e, stack) => Some (c0, e0, stack)
-    | (cCons (Access n) c, cons (c0,e0) e, stack) => Some (cCons (Access (n-1)) c, e, stack)
-    | (cCons (Push c) c0, e, stack) => Some (c0, e, cons (c,e) stack)
-    | (cCons Grab c, e, cons (c0,e0) stack) => Some (c, cons (c0,e0) e, stack)
-    | _ => None
+    | (cCons (Access 0) c, cons (c0,e0) e, stack) => (c0, e0, stack)
+    | (cCons (Access n) c, cons (c0,e0) e, stack) => (cCons (Access (n-1)) c, e, stack)
+    | (cCons (Push c) c0, e, stack) => (c0, e, cons (c,e) stack)
+    | (cCons Grab c, e, cons (c0,e0) stack) => (c, cons (c0,e0) e, stack)
+    | s => s
   end.
 
 (*Compiling*)
@@ -43,7 +44,7 @@ Fixpoint compile (t: term): code :=
   match t with
       | Var n => cCons (Access n) cnil
       | Lambda t1 => cCons Grab (compile t1)
-      | App t1 t2 => cCons (Push (compile t1)) (compile t2) 
+      | App t1 t2 => cCons (Push (compile t2)) (compile t1) 
   end.
 
 
@@ -55,14 +56,254 @@ Fixpoint tau_code (c: code): term :=
     | (cCons Grab c0) => Lambda (tau_code c0)
   end.
 
-Fixpoint tau_env (e: env): term :=
+Check multiple_substitution.
+
+Fixpoint tau_env (e: environment): list term :=
   match e with
-    | nul
-    |
-  end
+    | nul => nil
+    | cons (c0, e0) e1 =>
+      (multiple_substitution (tau_code c0) (tau_env e0) 0 (length (tau_env e0))) :: tau_env e1
+  end.
+
+Check state.
+
+Fixpoint transform_stk (stk: environment): term :=
+  match stk with
+      | cons (c0, e0) nul => multiple_substitution (tau_code c0) (tau_env e0) 0 (length (tau_env e0))
+      | cons (c0, e0) e1 => App (multiple_substitution (tau_code c0) (tau_env e0) 0 (length (tau_env e0))) (transform_stk e1)
+      | _ => Var 0
+  end.
+
+Fixpoint tau (s: state): term :=
+  match s with
+    | (c, e, stk) =>
+      match stk with
+        | nul => multiple_substitution (tau_code c) (tau_env e) 0 (length (tau_env e))
+        | stk => App (multiple_substitution (tau_code c) (tau_env e) 0 (length (tau_env e))) (transform_stk stk)
+      end
+  end.
+
+(*Compiling results*)
+
+
+Lemma tau_nil_env: forall t: term, tau (compile t, nul, nul) = tau_code (compile t).
+Proof.
+  induction t.
+  simpl.
+  have: beq_nat v v = true.
+  apply beq_nat_true_iff.
+  reflexivity.
+  intro h0.
+  rewrite h0.
+  rewrite -minus_n_O.
+  have: leb v 0 = false \/ leb v 0 = true.
+  apply dic.
+  intro h1.
+  case:h1.
+  intro h1.
+  rewrite h1.
+  trivial.
+  intro h1.
+  rewrite h1.
+  case v.
+  done.
+  done.
+  simpl.
+  rewrite -lambda_equivalence.
+  apply id_substitution.
+  simpl.
+  rewrite app_equivalence.
+  split.
+  apply id_substitution.
+  apply id_substitution.
+Qed.
+  
+Theorem invert_comp: forall (t: term), tau (compile t, nul, nul) = t.
+Proof.
+  induction t.
+  simpl.
+  have: beq_nat v v = true.
+  apply beq_nat_true_iff.
+  reflexivity.
+  intro h0.
+  rewrite h0.
+  rewrite -minus_n_O.
+  have: leb v 0 = false \/ leb v 0 = true.
+  apply dic.
+  intro h1.
+  case:h1.
+  intro h1.
+  rewrite h1.
+  trivial.
+  intro h1.
+  rewrite h1.
+  case v.
+  done.
+  done.
+  simpl.
+  rewrite -lambda_equivalence.
+  rewrite tau_nil_env in IHt.
+  rewrite IHt.
+  apply id_substitution.
+  simpl.
+  rewrite app_equivalence.
+  rewrite tau_nil_env in IHt1.
+  rewrite tau_nil_env in IHt2.
+  split.
+  rewrite IHt1.
+  apply id_substitution.
+  rewrite IHt2.
+  apply id_substitution.
+Qed.
+
+(*Correct state*)
+
+Fixpoint length (e: environment): nat :=
+  match e with
+    | nul => 0
+    | cons (c0, e0) e1 => 1 + (length e1)
+  end.
+
+Fixpoint correct_stk (stk: environment): Prop:=
+  match stk with
+    | nul => True
+    | cons (c0, e0) e => (correct_stk e0) /\ (correct_stk e) /\ (C (length e0) (tau_code c0)) 
+  end.
+
+Fixpoint correct_state (s: state): Prop:=
+  match s with
+   | (c, e, stk) => (correct_stk e) /\ (correct_stk stk) /\ (C (length e) (tau_code c))
+  end.
+
+Theorem transition_inv_1: forall (c c0: code) (e e0 stack: environment), correct_state ((cCons (Access 0) c, cons (c0,e0) e, stack)) -> correct_state  (c0, e0, stack).
+Proof.
+  simpl.
+  intros.
+  split.
+  apply H.
+  split.
+  apply H.
+  apply H.
+Qed.
+
+Theorem transition_inv_2: forall (c c0: code) (e e0 stack: environment) (n: nat), (n > 0) -> correct_state (cCons (Access n) c, cons (c0,e0) e, stack) -> correct_state (cCons (Access (n-1)) c, e, stack).
+Proof.
+  simpl.
+  intros.
+  split.  
+  apply H0.
+  split.
+  apply H0.
+  destruct H0.
+  destruct H1.
+  omega.
+Qed.
+
+Theorem transition_inv_3: forall (c c0: code) (e stack: environment), correct_state (cCons (Push c) c0, e, stack) -> correct_state (c0, e, cons (c,e) stack).
+Proof.
+  simpl.  
+  intros.
+  split.
+  apply H.
+  split.
+  split.
+  apply H.
+  split.
+  apply H.
+  apply H.
+  apply H.  
+Qed.
+
+Theorem transition_inv_4: forall (c c0: code) (e e0 stack: environment), correct_state (cCons Grab c, e, cons (c0,e0) stack) -> correct_state (c, cons (c0,e0) e, stack).
+Proof.
+  simpl.
+  intros.
+  split.
+  split.
+  apply H.
+  split.
+  apply H.
+  apply H.
+  split.
+  apply H.
+  rewrite plus_comm in H.
+  apply H.
+Qed.
+
+Theorem correct_invariance: forall s: state, correct_state s -> correct_state (exec_inst s).
+Proof.
+  intro.
+  destruct s.
+  destruct p.
+  move: e e0.
+  induction c.
+  move => e e0.
+  case e0.
+  case e.
+  simpl.
+  done.
+  simpl.
+  done.
+  simpl.
+  done.
+  case i.
+  intros n e e0.
+  case e0.
+  case n.
+  simpl.
+  done.
+  simpl.
+  done.
+  intros p e1.
+  destruct p.
+  unfold exec_inst.
+  case n.
+  apply transition_inv_1.
+  intro.
+  apply transition_inv_2.
+  omega.
+  unfold exec_inst.
+  intros e e0.
+  case e.
+  done.
+  intros p e1.
+  destruct p.
+  apply transition_inv_4.
+  intros c0 e e0.
+  apply transition_inv_3.
+Qed.
+
+Lemma toy_lemma: forall (c c0: code) (e s: environment), correct_state (cCons (Push c0) c,e,s) -> reduces (tau (cCons (Push c0) c,e,s)) (tau (c, e, cons (c0, e) s)).
+Proof.
+  intros.
+  simpl.
+  case s.
+  apply sym.
+  intros.
+  destruct p.
+  apply red_equivalence.
+  exists 0.
+  simpl.
+  done.
+Qed.
+
+Theorem correct_confluence: forall s: state, correct_state s -> reduces (tau s) (tau (exec_inst s)).
+Proof.
+  induction s.
+  destruct a.
+  simpl.
+
+
+
+  (*Unify every transition*)
 
 
 
 
 
 
+
+
+
+
+  
